# 51. (kk|ɛ)((kg)+g)*g(gk)*

- e0 = ε
- e1 = kk
- e2 = kg
- e3 = g
- e4 = gk
<hr>
- S0 -> ε
- S1 -> kk
- S2 -> kg
- S3 -> g
- S4 -> gk

### Далі обробимо складніші конструкції:

#### 1. (kg) + g:

- S5 -> S2 S6
- S6 -> S2 S6 | S3

#### 2. ((kg) + g)*:

- S7 -> S5 | ε
- S5 -> S2 S6
- S6 -> S2 S6 | S3

#### 3. g(gk)*:

- S8 -> S3 S9
- S9 -> S4 S9 | ε
- S3 -> g
- S4 -> gk

### Збираємо всі частини в одній граматиці:

(kk | ε):

- S10 -> S1 | S0

### Загальне правило для (kk|ε)((kg)+g)*g(gk)*

- S -> S10 S7 S8
- S10 -> S1 | S0
- S1 -> kk
- S0 -> ε
- S7 -> S5 | ε
- S5 -> S2 S6
- S6 -> S2 S6 | S3
- S2 -> kg
- S3 -> g
- S8 -> S3 S9
S9 -> S4 S9 | ε
S4 -> gk
